theories/imp_to_asm.v
@@ -115,12 +115,10 @@ Definition touched_registers : list string :=
   tmp_registers ++ saved_registers.
 
 Definition i2a_regs_call (ret : Z) (rs : gmap string Z) : Prop :=
-  rs !! "R30" = Some ret ∧
-  map_list_included touched_registers rs.
+  rs !!! "R30" = ret.
 
 Definition i2a_regs_ret (rs rsold : gmap string Z) (av : Z) : Prop :=
   rs !!! "R0" = av ∧
-  map_list_included touched_registers rs ∧
   map_preserved saved_registers rsold rs.
 
 (** ** mapping of provenances *)
@@ -663,13 +661,12 @@ Definition i2a_heap_inv (h : heap_state) : uPred imp_to_asmUR :=
          i2a_heap_shared_agree (h_heap h) ih ∗ i2a_heap_auth ih.
 
 Definition i2a_args (o : nat) (vs : list val) (rs : gmap string Z) : uPred imp_to_asmUR :=
-  ([∗ list] i↦v∈vs, ∃ r av,
+  ([∗ list] i↦v∈vs, ∃ r,
       ⌜args_registers !! (o + i)%nat = Some r⌝ ∗
-      ⌜rs !! r = Some av⌝ ∗
-      i2a_val_rel v av).
+      i2a_val_rel v (rs !!! r)).
 
 Definition i2a_args_pure (o : nat) (vs : list Z) (rs : gmap string Z) : Prop :=
-  ∀ i v, vs !! i = Some v → ∃ r, args_registers !! (o + i)%nat = Some r ∧ rs !! r = Some v.
+  ∀ i v, vs !! i = Some v → ∃ r, args_registers !! (o + i)%nat = Some r ∧ rs !!! r = v.
 
 Lemma i2a_mem_uninit_split n a l :
   0 ≤ n ≤ l →
@@ -1095,7 +1092,7 @@ Lemma i2a_args_nil o rs:
 Proof. done. Qed.
 
 Lemma i2a_args_cons1 o v vs rs:
-  i2a_args o (v::vs) rs ⊣⊢ (∃ av r, ⌜args_registers !! o = Some r⌝ ∗ ⌜rs !! r = Some av⌝ ∗ i2a_val_rel v av) ∗ i2a_args (S o) vs rs.
+  i2a_args o (v::vs) rs ⊣⊢ (∃ r, ⌜args_registers !! o = Some r⌝ ∗ i2a_val_rel v (rs !!! r)) ∗ i2a_args (S o) vs rs.
 Proof.
   rewrite /i2a_args. setoid_rewrite Nat.add_succ_l. setoid_rewrite <-Nat.add_succ_r => /=.
   f_equiv. setoid_rewrite Nat.add_0_r. iSplit; iIntros!; iSplit!.
@@ -1103,7 +1100,7 @@ Qed.
 
 Lemma i2a_args_cons o v vs rs r:
   args_registers !! o = Some r →
-  i2a_args o (v::vs) rs ⊣⊢ (∃ av, ⌜rs !! r = Some av⌝ ∗ i2a_val_rel v av) ∗ i2a_args (S o) vs rs.
+  i2a_args o (v::vs) rs ⊣⊢ i2a_val_rel v (rs !!! r) ∗ i2a_args (S o) vs rs.
 Proof. move => ?. rewrite i2a_args_cons1. iSplit; iIntros!; iSplit!. Qed.
 
 Lemma i2a_args_mono o vs rs rs':
@@ -1112,8 +1109,8 @@ Lemma i2a_args_mono o vs rs rs':
   i2a_args o vs rs'.
 Proof.
   iIntros (Hpre) "Hargs". iApply (big_sepL_impl with "Hargs").
-  iIntros "!>" (???) "[% [% [% [% ?]]]]". iExists _, _. iFrame. iSplit; [done|]. iPureIntro.
-  etrans; [symmetry; apply: Hpre|done].
+  iIntros "!>" (???) "[% [% ?]]". iExists _. iFrame. iSplit; [done|].
+  rewrite ->Hpre; [done|].
   apply elem_of_list_lookup. setoid_rewrite lookup_drop. naive_solver.
 Qed.
 
@@ -1125,7 +1122,7 @@ Proof.
   iIntros (Hpure) "Hvs".
   iInduction vs as [|v vs] "IH" forall (avs o Hpure). { by rewrite i2a_args_nil. }
   iDestruct (big_sepL2_cons_inv_l with "Hvs") as (???) "[??]". simplify_eq.
-  have [?[]]:= Hpure 0%nat _ ltac:(done). rewrite Nat.add_0_r => ??.
+  have [?[]]:= Hpure 0%nat _ ltac:(done). rewrite Nat.add_0_r => ??. simplify_eq.
   rewrite i2a_args_cons; [|done].
   iDestruct ("IH" with "[%] [$]") as "$". 2: by iSplit!.
   move => ???. rewrite Nat.add_succ_l -Nat.add_succ_r. by apply Hpure.
@@ -1448,7 +1445,7 @@ Lemma imp_to_asm_proof ins fns ins_dom fns_dom f2i :
   ins_dom = dom _ ins →
   fns_dom = dom _ fns →
   (∀ n i rs mem K f fn vs h cs pc ret gp rf rc lr,
-      rs !! "PC" = Some pc →
+      rs !!! "PC" = pc →
       ins !! pc = Some i →
       fns !! f = Some fn →
       f2i !! f = Some pc →
@@ -1459,7 +1456,7 @@ Lemma imp_to_asm_proof ins fns ins_dom fns_dom f2i :
       (* Call *)
       (∀ K' rs' mem' f' es vs pc' ret' gp' h' lr' rf' r',
           Forall2 (λ e v, e = Val v) es vs →
-          rs' !! "PC" = Some pc' →
+          rs' !!! "PC" = pc' →
           (ins !! pc' = None ↔ fns !! f' = None) →
           f2i !! f' = Some pc' →
           satisfiable (i2a_mem_inv (rs' !!! "SP") gp' mem' ∗ i2a_heap_inv h' ∗
@@ -1468,7 +1465,7 @@ Lemma imp_to_asm_proof ins fns ins_dom fns_dom f2i :
           is_Some (ins !! ret') →
           map_scramble touched_registers lr' rs' →
           (∀ rs'' mem'' av v h'' rf'' lr'',
-              rs'' !! "PC" = Some ret' →
+              rs'' !!! "PC" = ret' →
               satisfiable (i2a_mem_inv (rs'' !!! "SP") gp' mem'' ∗ i2a_heap_inv h'' ∗
                            i2a_val_rel v av ∗ rf'' ∗ r') →
               i2a_regs_ret rs'' rs' av →
@@ -1479,7 +1476,7 @@ Lemma imp_to_asm_proof ins fns ins_dom fns_dom f2i :
                (SMProg, Imp (expr_fill K (expr_fill K' (imp.Call f' es))) h' fns, (PPInside, I2A cs lr', rf'))) →
       (* Return *)
       (∀ rs' mem' av v h' lr' rf',
-          rs' !! "PC" = Some ret →
+          rs' !!! "PC" = ret →
           satisfiable (i2a_mem_inv (rs' !!! "SP") gp mem' ∗ i2a_heap_inv h' ∗
                       i2a_val_rel v av ∗ rf' ∗ rc) →
           i2a_regs_ret rs' rs av →
@@ -1510,7 +1507,7 @@ Proof.
   { simpl. exact (λ  '(AsmState i1 rs1 mem1 ins'1) '(σfs1, Imp e1 h1 fns'1, (t1, I2A cs1 lr1, r1))
                      '(AsmState i2 rs2 mem2 ins'2) '(σfs2, Imp e2 h2 fns'2, (t2, I2A cs2 lr2, r2)),
     ∃ i K av v pc lr' gp,
-      rs2 !! "PC" = Some pc ∧
+      rs2 !!! "PC" = pc ∧
       ins !! pc = Some i ∧
       satisfiable (i2a_mem_inv (rs2 !!! "SP") gp mem2 ∗ i2a_heap_inv h2 ∗ i2a_val_rel v av ∗ r1 ∗ r2) ∧
       i2a_regs_ret rs2 lr' av ∧
@@ -1537,7 +1534,7 @@ Proof.
     Hf both for calls triggered from inside and outside the module. *)
     unshelve eapply tsim_remember. { exact (λ n '(AsmState i1 rs1 mem1 ins'1) '(σfs1, Imp e1 h1 fns'1, (t1, I2A cs1 lr1, r1)),
        ∃ K' pc i ret f fn vs r' gp,
-         rs1 !! "PC" = Some pc ∧
+         rs1 !!! "PC" = pc ∧
          ins !! pc = Some i ∧
          fns !! f = Some fn ∧
          f2i !! f = Some pc ∧
@@ -1553,7 +1550,7 @@ Proof.
          t1 = PPInside ∧
          σfs1 = SMProg ∧
          (∀ rs' mem' av v h' lr' rf',
-          rs' !! "PC" = Some ret →
+          rs' !!! "PC" = ret →
           satisfiable (i2a_mem_inv (rs' !!! "SP") gp mem' ∗ i2a_heap_inv h' ∗
                       i2a_val_rel v av ∗ r' ∗ rf') →
           i2a_regs_ret rs' rs1 av  →
@@ -1569,16 +1566,16 @@ Proof.
       tstep_s. split!. { instantiate (1:=[_]). done. } { iSatMono. iIntros!. iFrame. iAccu. }
       apply Hstay; [done|]. by split!.
     }
-    { move => ?? [????] [[?[???]][[?[??]]?]] ??. destruct_all?. split!; [done..|].
+    { move => ?? [????] [[?[???]][[?[??]]?]] ??. destruct_all?. simplify_eq. split!; [done..|].
       move => *. apply: tsim_mono; [naive_solver|]. etrans; [|done]. apply ti_le_S. }
     iSatClear.
     move => n' /= Hn' IH [i' rs' mem' ins'] [[?[???]][[?[??]]?]] ?. destruct_all?; simplify_eq.
-    apply: Hf; [try eassumption..| |].
+    apply: Hf; [try done..| |].
     { iSatMono. iIntros!. iFrame. iAccu. }
     + iSatClear.
       move => K'' rs'' mem'' f'' es vs'' pc'' ret'' gp'' h'' lr rf'' r'' Hall ??????? Hret'.
       have ?: es = Val <$> vs''. { clear -Hall. elim: Hall; naive_solver. } subst.
-      destruct (ins !! pc'') eqn:Hi.
+      destruct (ins !! (rs'' !!! "PC")) eqn:Hi.
       * have [??] : is_Some (fns !! f''). { apply not_eq_None_Some. naive_solver. }
         tstep_s. left. split! => ?/=.
         apply IH; [done|]. split! => //.
